Untitled
================
ActuarialCat

![
Z = \\frac{N}{N + K} = \\frac{\\text{Va}r\_{\\Theta}\\left( \\mu\\left( \\Theta \\right) \\right)}{\\text{Var}\\left( \\overline{X} \\right)}
](https://latex.codecogs.com/png.latex?%0AZ%20%3D%20%5Cfrac%7BN%7D%7BN%20%2B%20K%7D%20%3D%20%5Cfrac%7B%5Ctext%7BVa%7Dr_%7B%5CTheta%7D%5Cleft%28%20%5Cmu%5Cleft%28%20%5CTheta%20%5Cright%29%20%5Cright%29%7D%7B%5Ctext%7BVar%7D%5Cleft%28%20%5Coverline%7BX%7D%20%5Cright%29%7D%0A "
Z = \frac{N}{N + K} = \frac{\text{Va}r_{\Theta}\left( \mu\left( \Theta \right) \right)}{\text{Var}\left( \overline{X} \right)}
")

![
\\widehat{\\text{EPV}} = \\frac{\\sum\_{i = 1}^{R}{\\sum\_{t = 1}^{N\_{i}}{m\_{\\text{it}\\ }\\left( X\_{\\text{it}} - {\\overline{X}}\_{i} \\right)}^{2}}}{\\sum\_{i = 1}^{R}\\left( N\_{i} - 1 \\right)}
](https://latex.codecogs.com/png.latex?%0A%5Cwidehat%7B%5Ctext%7BEPV%7D%7D%20%3D%20%5Cfrac%7B%5Csum_%7Bi%20%3D%201%7D%5E%7BR%7D%7B%5Csum_%7Bt%20%3D%201%7D%5E%7BN_%7Bi%7D%7D%7Bm_%7B%5Ctext%7Bit%7D%5C%20%7D%5Cleft%28%20X_%7B%5Ctext%7Bit%7D%7D%20-%20%7B%5Coverline%7BX%7D%7D_%7Bi%7D%20%5Cright%29%7D%5E%7B2%7D%7D%7D%7B%5Csum_%7Bi%20%3D%201%7D%5E%7BR%7D%5Cleft%28%20N_%7Bi%7D%20-%201%20%5Cright%29%7D%0A "
\widehat{\text{EPV}} = \frac{\sum_{i = 1}^{R}{\sum_{t = 1}^{N_{i}}{m_{\text{it}\ }\left( X_{\text{it}} - {\overline{X}}_{i} \right)}^{2}}}{\sum_{i = 1}^{R}\left( N_{i} - 1 \right)}
")

![
\\widehat{\\text{VHM}} = \\frac{\\left( \\sum\_{i = 1}^{R}{m\_{i}\\left( {\\overline{X}}\_{i} - \\overline{X} \\right)^{2}} \\right) - \\left( R - 1 \\right)\\widehat{\\text{EPV}}}{m - \\frac{1}{m}\\sum\_{i = 1}^{R}m\_{i}^{2}}
](https://latex.codecogs.com/png.latex?%0A%5Cwidehat%7B%5Ctext%7BVHM%7D%7D%20%3D%20%5Cfrac%7B%5Cleft%28%20%5Csum_%7Bi%20%3D%201%7D%5E%7BR%7D%7Bm_%7Bi%7D%5Cleft%28%20%7B%5Coverline%7BX%7D%7D_%7Bi%7D%20-%20%5Coverline%7BX%7D%20%5Cright%29%5E%7B2%7D%7D%20%5Cright%29%20-%20%5Cleft%28%20R%20-%201%20%5Cright%29%5Cwidehat%7B%5Ctext%7BEPV%7D%7D%7D%7Bm%20-%20%5Cfrac%7B1%7D%7Bm%7D%5Csum_%7Bi%20%3D%201%7D%5E%7BR%7Dm_%7Bi%7D%5E%7B2%7D%7D%0A "
\widehat{\text{VHM}} = \frac{\left( \sum_{i = 1}^{R}{m_{i}\left( {\overline{X}}_{i} - \overline{X} \right)^{2}} \right) - \left( R - 1 \right)\widehat{\text{EPV}}}{m - \frac{1}{m}\sum_{i = 1}^{R}m_{i}^{2}}
")
